# Interpreter-Project

### BNF

```
// Grammar 0 in BNF: ( Original )
// <E>        ::= <T> <Eopt>
// <Eopt>     ::= "+" <T> <Eopt> | "-" <T> <Eopt> | <empty>
// <T>        ::= <NR> <Topt>
// <Topt>     ::= "*" <NR> <Topt> | "/" <NR> <Topt> | <empty>
// <NR>       ::= "Num" <value> | "(" <E> ")"

// Grammar 1 in BNF:
// <E>        ::= <T> <Eopt>
// <Eopt>     ::= "+" <T> <Eopt> | "-" <T> <Eopt> | <empty>
// <T>        ::= <NR> <Topt>
// <Topt>     ::= "*" <NR> <Topt> | "/" <NR> <Topt> | "%" <NR> <Topt> | <empty>
// <NR>       ::= "Num" <value> | "(" <E> ")"

// Grammar 2 in BNF:
// <E>        ::= <T> <Eopt>
// <Eopt>     ::= "+" <T> <Eopt> | "-" <T> <Eopt> | <empty>
// <T>        ::= <P> <Topt>
// <Topt>     ::= "*" <NR> <Topt> | "/" <NR> <Topt> | "%" <NR> <Topt> | <empty>
// <P>        ::= <NR> <Popt>                 
// <Popt>     ::= "^" <NR> <Popt> | <empty>
// <NR>       ::= "Num" <value> | "(" <E> ")"

// Updated Grammar 3 in BNF:
// <E>        ::= <T> <Eopt>
// <Eopt>     ::= "+" <T> <Eopt> | "-" <T> <Eopt> | <empty>
// <T>        ::= <P> <Topt>
// <Topt>     ::= "*" <P> <Topt> | "/" <P> <Topt> | "%" <P> <Topt> | <empty>
// <P>        ::= <U> <Popt>
// <Popt>     ::= "^" <U> <Popt> | <empty>
// <U>        ::= "-" <U> | <NR>
// <NR>       ::= "Num" <value> | "(" <E> ")"

// Updated Grammar 4 in BNF: ( Current )
// <E>        ::= <T> <Eopt>
// <Eopt>     ::= "+" <T> <Eopt> | "-" <T> <Eopt> | <empty>
// <T>        ::= <P> <Topt>
// <Topt>     ::= "*" <P> <Topt> | "/" <P> <Topt> | "%" <P> <Topt> | <empty>
// <P>        ::= <U> <Popt>
// <Popt>     ::= "^" <U> <Popt> | <empty>
// <U>        ::= "-" <U> | <NM>
// <NM>       ::= <IN> | <FL> | "(" <E> ")"
// <IN>       ::= <digit>+
// <FL>       ::= <digit>+ "." <digit>+

// E    -> Expression
// Eopt -> Expression/Optional
// T    -> Term
// Topt -> Term/Optional
// P    -> Power
// Popt -> Power/Optional
// U    -> Unary
// FL   -> Floating Point
// NM   -> Number
// IN   -> Integer
// FL   -> Float
```
